@prefix : <https://w3id.org/sebi#> .
@prefix owl: <http://www.w3.org/2002/07/owl#> .
@prefix rdf: <http://www.w3.org/1999/02/22-rdf-syntax-ns#> .
@prefix xml: <http://www.w3.org/XML/1998/namespace> .
@prefix xsd: <http://www.w3.org/2001/XMLSchema#> .
@prefix rdfs: <http://www.w3.org/2000/01/rdf-schema#> .
@base <https://w3id.org/sebi#> .

<https://w3id.org/sebi> rdf:type owl:Ontology ;
                         owl:versionIRI <https://w3id.org/sebi/version/2024-06-04> .

#################################################################
#    Object Properties
#################################################################

###  https://w3id.org/sebi/assess
<https://w3id.org/sebi/assess> rdf:type owl:ObjectProperty ;
                               rdfs:domain <https://w3id.org/sebi/Evidence> ;
                               rdfs:range <https://w3id.org/sebi/Feature> ;
                               rdfs:comment "A relationship indicating that an Evidence examines a Feature (e.g. the evidence assess (or examines) the style of the document)." ;
                               rdfs:label "assess" .


###  https://w3id.org/sebi/evaluate
<https://w3id.org/sebi/evaluate> rdf:type owl:ObjectProperty ;
                                 rdfs:domain <https://w3id.org/sebi/Evidence> ;
                                 rdfs:range <https://w3id.org/sebi/Evaluation> ;
                                 rdfs:comment "A relationship indicating that an Evidence gives an Evaluation when evaluating a Feature (e.g. the evidence evaluates the **presence** of interpolations)." ;
                                 rdfs:label "evaluate" .


###  https://w3id.org/sebi/hasEvaluation
<https://w3id.org/sebi/hasEvaluation> rdf:type owl:ObjectProperty ;
                                      owl:inverseOf <https://w3id.org/sebi/hasFeature> ;
                                      rdfs:domain <https://w3id.org/sebi/Feature> ;
                                      rdfs:range <https://w3id.org/sebi/Evaluation> ;
                                      rdfs:comment "A relationship indicating the Evaluation associated with a Feature (e.g. the presence of interpolations). Inverse proprty of has feature." ;
                                      rdfs:label "has evaluation" .


###  https://w3id.org/sebi/hasFeature
<https://w3id.org/sebi/hasFeature> rdf:type owl:ObjectProperty ;
                                   rdfs:domain <https://w3id.org/sebi/Evaluation> ;
                                   rdfs:range <https://w3id.org/sebi/Feature> ;
                                   rdfs:comment "A relationship indicating the Feature to which an Evaluation is associated (e.g. interpolations are present in the document)." ;
                                   rdfs:label "has feature" .


###  https://w3id.org/sebi/intend
<https://w3id.org/sebi/intend> rdf:type owl:ObjectProperty ;
                               owl:inverseOf <https://w3id.org/sebi/intendedTo> ;
                               rdfs:domain <https://w3id.org/sebi/Intention> ;
                               rdfs:range <https://w3id.org/sebi/Document> ;
                               rdfs:comment "A relationship indicating which document has been created with a certain Intention. Inverse proprty of intend. " ;
                               rdfs:label "intend" .


###  https://w3id.org/sebi/intendedTo
<https://w3id.org/sebi/intendedTo> rdf:type owl:ObjectProperty ;
                                   rdfs:domain <https://w3id.org/sebi/Document> ;
                                   rdfs:range <https://w3id.org/sebi/Intention> ;
                                   rdfs:comment "A relationship indicating the Intention with which a document has been created (e.g. for profit purposes)." ;
                                   rdfs:label "intended to" .


###  https://w3id.org/sebi/isAssessedBy
<https://w3id.org/sebi/isAssessedBy> rdf:type owl:ObjectProperty ;
                                     owl:inverseOf <https://w3id.org/sebi/assess> ;
                                     rdfs:domain <https://w3id.org/sebi/Feature> ;
                                     rdfs:range <https://w3id.org/sebi/Evidence> ;
                                     rdfs:comment "A relationship indicating that a Feature is examined in an Evidence (e.g. the style of the document is assessed (or examined) in the evidence). Inverse property of assess." ;
                                     rdfs:label "is assessed by" .


###  https://w3id.org/sebi/isEvaluatedBy
<https://w3id.org/sebi/isEvaluatedBy> rdf:type owl:ObjectProperty ;
                                      owl:inverseOf <https://w3id.org/sebi/evaluate> ;
                                      rdfs:domain <https://w3id.org/sebi/Evaluation> ;
                                      rdfs:range <https://w3id.org/sebi/Evidence> ;
                                      rdfs:comment "A relationship indicating that an Evaluation is given in an Evidence when evaluating a Feature  (e.g. **presence** of interpolations has been evaluated in the evidence). Inverse property of evaluate. " ;
                                      rdfs:label "is evaluated by" .


###  https://w3id.org/sebi/isSupportedBy
<https://w3id.org/sebi/isSupportedBy> rdf:type owl:ObjectProperty ;
                                      owl:inverseOf <https://w3id.org/sebi/support> ;
                                      rdfs:domain <https://w3id.org/hico#InterpretationAct> ;
                                      rdfs:range <https://w3id.org/sebi/Evidence> ;
                                      rdfs:comment "A relationship indicating that an Interpretation is supported by an Evidence. Inverse property of support" ;
                                      rdfs:label "is supported by" .


###  https://w3id.org/sebi/support
<https://w3id.org/sebi/support> rdf:type owl:ObjectProperty ;
                                rdfs:domain <https://w3id.org/sebi/Evidence> ;
                                rdfs:range <https://w3id.org/hico#InterpretationAct> ;
                                rdfs:comment "A relationship indicating that an Evidence supports an Interpretation." ;
                                rdfs:label "support" .


#################################################################
#    Data properties
#################################################################

###  https://w3id.org/sebi/hasEvaluationScore
<https://w3id.org/sebi/hasEvaluationScore> rdf:type owl:DatatypeProperty ;
                                           rdfs:domain <https://w3id.org/sebi/Evidence> ;
                                           rdfs:range xsd:integer ;
                                           rdfs:comment "The evaluation score given to an Evidence to register its polarity (e.g. score 0 on consistency means inconsistent, score 1 means consintent)" ;
                                           rdfs:label "has evaluation score" .


#################################################################
#    Classes
#################################################################

###  https://w3id.org/hico#InterpretationAct
<https://w3id.org/hico#InterpretationAct> rdf:type owl:Class .


###  https://w3id.org/sebi/Authentic
<https://w3id.org/sebi/Authentic> rdf:type owl:Class ;
                                  rdfs:subClassOf <https://w3id.org/sebi/Document> ;
                                  rdfs:comment "An authentic document is a document which is believed to be genuine" ;
                                  rdfs:label "Authentic document" .


###  https://w3id.org/sebi/Document
<https://w3id.org/sebi/Document> rdf:type owl:Class ;
                                 owl:disjointWith <https://w3id.org/sebi/Evaluation> ,
                                                  <https://w3id.org/sebi/Evidence> ,
                                                  <https://w3id.org/sebi/Feature> ,
                                                  <https://w3id.org/sebi/Intention> ;
                                 rdfs:comment "A document is a recorded piece of information, typically in written, that serves as device to communicate" ;
                                 rdfs:label "Document" .


###  https://w3id.org/sebi/Evaluation
<https://w3id.org/sebi/Evaluation> rdf:type owl:Class ;
                                   owl:disjointWith <https://w3id.org/sebi/Evidence> ,
                                                    <https://w3id.org/sebi/Feature> ,
                                                    <https://w3id.org/sebi/Intention> ;
                                   rdfs:comment "A specific quality or feature detected in an evidence (e.g. reliability, completeness)" ;
                                   rdfs:label "Evaluation" .


###  https://w3id.org/sebi/Evidence
<https://w3id.org/sebi/Evidence> rdf:type owl:Class ;
                                 owl:disjointWith <https://w3id.org/sebi/Feature> ,
                                                  <https://w3id.org/sebi/Intention> ;
                                 rdfs:comment "A piece of evidence or proof used in the investigation" ;
                                 rdfs:label "Evidence" .


###  https://w3id.org/sebi/ExtrinsicFeature
<https://w3id.org/sebi/ExtrinsicFeature> rdf:type owl:Class ;
                                         rdfs:subClassOf <https://w3id.org/sebi/Feature> ;
                                         rdfs:comment "An external characteristic of a document, such as ink or paper" ;
                                         rdfs:label "Extrinsic feature" .


###  https://w3id.org/sebi/Feature
<https://w3id.org/sebi/Feature> rdf:type owl:Class ;
                                owl:disjointWith <https://w3id.org/sebi/Intention> ;
                                rdfs:comment "A characteristic or Evaluation of a document on which an evidence is based on (e.g. style, language)" ;
                                rdfs:label "Feature" .


###  https://w3id.org/sebi/Forgery
<https://w3id.org/sebi/Forgery> rdf:type owl:Class ;
                                rdfs:subClassOf <https://w3id.org/sebi/Document> ;
                                rdfs:comment "A forgery is a document intentionally created or altered with the intent to deceive or defraud by passing it off as genuine" ;
                                rdfs:label "Forgery" .


###  https://w3id.org/sebi/Intention
<https://w3id.org/sebi/Intention> rdf:type owl:Class ;
                                  rdfs:comment "An intention is the purpose that led to the creation of a document" ;
                                  rdfs:label "Intention" .


###  https://w3id.org/sebi/IntrinsicFeature
<https://w3id.org/sebi/IntrinsicFeature> rdf:type owl:Class ;
                                         rdfs:subClassOf <https://w3id.org/sebi/Feature> ;
                                         rdfs:comment "An internal characteristic of a document, such as style or content" ;
                                         rdfs:label "Intrinsic feature" .


###  https://w3id.org/sebi/Provenance
<https://w3id.org/sebi/Provenance> rdf:type owl:Class ;
                                   rdfs:subClassOf <https://w3id.org/sebi/Feature> ;
                                   rdfs:comment "The history of ownership and transmission of a document" ;
                                   rdfs:label "Provenance" .


###  https://w3id.org/sebi/SuspectedForgery
<https://w3id.org/sebi/SuspectedForgery> rdf:type owl:Class ;
                                         rdfs:subClassOf <https://w3id.org/sebi/Document> ;
                                         rdfs:comment "A suspected forgery is a document that is believed to be a result of forgery, but its authenticity has not been confirmed." ;
                                         rdfs:label "Supected forged document" .


#################################################################
#    Individuals
#################################################################

###  https://w3id.org/sebi/attendibility
<https://w3id.org/sebi/attendibility> rdf:type owl:NamedIndividual ,
                                               <https://w3id.org/sebi/Evaluation> ;
                                      rdfs:comment "The reliability of a document's content and the trustworthiness of its source." ;
                                      rdfs:label "attendibility" .


###  https://w3id.org/sebi/authentication_marks
<https://w3id.org/sebi/authentication_marks> rdf:type owl:NamedIndividual ,
                                                      <https://w3id.org/sebi/ExtrinsicFeature> ;
                                             rdfs:comment "Legal authentication marks or signs on a document that indicate its authenticity." ;
                                             rdfs:label "authentication marks" .


###  https://w3id.org/sebi/chronology_and_dating
<https://w3id.org/sebi/chronology_and_dating> rdf:type owl:NamedIndividual ,
                                                       <https://w3id.org/sebi/IntrinsicFeature> ;
                                              rdfs:comment "The timeline and historical context of a document" ;
                                              rdfs:label "chronology and dating" .


###  https://w3id.org/sebi/completeness
<https://w3id.org/sebi/completeness> rdf:type owl:NamedIndividual ,
                                              <https://w3id.org/sebi/Evaluation> ;
                                     rdfs:comment "The state of a document having all necessary parts or elements" ;
                                     rdfs:label "completeness" .


###  https://w3id.org/sebi/consistency
<https://w3id.org/sebi/consistency> rdf:type owl:NamedIndividual ,
                                             <https://w3id.org/sebi/Evaluation> ;
                                    rdfs:comment "The degree to which different parts of a document agree with each other" ;
                                    rdfs:label "consistency" .


###  https://w3id.org/sebi/content
<https://w3id.org/sebi/content> rdf:type owl:NamedIndividual ,
                                         <https://w3id.org/sebi/IntrinsicFeature> ;
                                rdfs:comment "The actual information or text contained in a document" ;
                                rdfs:label "content" .


###  https://w3id.org/sebi/document_provenance
<https://w3id.org/sebi/document_provenance> rdf:type owl:NamedIndividual ,
                                                     <https://w3id.org/sebi/Provenance> ;
                                            rdfs:comment "The documented history of a document's ownership and transmission" ;
                                            rdfs:label "document provenance" .


###  https://w3id.org/sebi/format_spacing_signs
<https://w3id.org/sebi/format_spacing_signs> rdf:type owl:NamedIndividual ,
                                                      <https://w3id.org/sebi/IntrinsicFeature> ;
                                             rdfs:comment "The layout, spacing, and sign usage in a document" ;
                                             rdfs:label "format (spacing, signs)" .


###  https://w3id.org/sebi/handwriting
<https://w3id.org/sebi/handwriting> rdf:type owl:NamedIndividual ,
                                             <https://w3id.org/sebi/ExtrinsicFeature> ;
                                    rdfs:comment "The style and characteristics of writing in a document" ;
                                    rdfs:label "handwriting" .


###  https://w3id.org/sebi/historical_context
<https://w3id.org/sebi/historical_context> rdf:type owl:NamedIndividual ,
                                                    <https://w3id.org/sebi/Provenance> ;
                                           rdfs:comment "The historical setting and background of a document" ;
                                           rdfs:label "historical context" .


###  https://w3id.org/sebi/historical_revisionism
<https://w3id.org/sebi/historical_revisionism> rdf:type owl:NamedIndividual ,
                                                        <https://w3id.org/sebi/Intention> ;
                                               rdfs:comment "The deliberate alteration or reinterpretation of historical records to reflect a specific agenda, often to legitimize or support a particular viewpoint." ;
                                               rdfs:label "historical revisionism" .


###  https://w3id.org/sebi/illustration
<https://w3id.org/sebi/illustration> rdf:type owl:NamedIndividual ,
                                              <https://w3id.org/sebi/IntrinsicFeature> ;
                                     rdfs:comment "Visual elements in a document, such as drawings or decorations" ;
                                     rdfs:label "illustration or other graphical device" .


###  https://w3id.org/sebi/indentation
<https://w3id.org/sebi/indentation> rdf:type owl:NamedIndividual ,
                                             <https://w3id.org/sebi/ExtrinsicFeature> ;
                                    rdfs:comment "Impressions left on a document from writing or sealing" ;
                                    rdfs:label "indentation" .


###  https://w3id.org/sebi/ink
<https://w3id.org/sebi/ink> rdf:type owl:NamedIndividual ,
                                     <https://w3id.org/sebi/ExtrinsicFeature> ;
                            rdfs:comment "The type and composition of ink used in a document" ;
                            rdfs:label "ink" .


###  https://w3id.org/sebi/inter_punctuation
<https://w3id.org/sebi/inter_punctuation> rdf:type owl:NamedIndividual ,
                                                   <https://w3id.org/sebi/IntrinsicFeature> ;
                                          rdfs:comment "The punctuation used between words and sentences" ;
                                          rdfs:label "inter-punctuation" .


###  https://w3id.org/sebi/interpolations
<https://w3id.org/sebi/interpolations> rdf:type owl:NamedIndividual ,
                                                <https://w3id.org/sebi/IntrinsicFeature> ;
                                       rdfs:comment "Additional text inserted into a document after its original creation, often indicating tampering." ;
                                       rdfs:label "interpolations" .


###  https://w3id.org/sebi/legal_formulas
<https://w3id.org/sebi/legal_formulas> rdf:type owl:NamedIndividual ,
                                                <https://w3id.org/sebi/ExtrinsicFeature> ;
                                       rdfs:comment "Standard legal phrases or formats in a document" ;
                                       rdfs:label "legal formulas" .


###  https://w3id.org/sebi/list_of_witnesses
<https://w3id.org/sebi/list_of_witnesses> rdf:type owl:NamedIndividual ,
                                                   <https://w3id.org/sebi/Provenance> ;
                                          rdfs:comment "A record of individuals who have seen or authenticated a documents" ;
                                          rdfs:label "list of witnesses" .


###  https://w3id.org/sebi/material_support
<https://w3id.org/sebi/material_support> rdf:type owl:NamedIndividual ,
                                                  <https://w3id.org/sebi/ExtrinsicFeature> ;
                                         rdfs:comment "The material on which a document is written, such as paper or parchment" ;
                                         rdfs:label "material support" .


###  https://w3id.org/sebi/metre_and_style
<https://w3id.org/sebi/metre_and_style> rdf:type owl:NamedIndividual ,
                                                 <https://w3id.org/sebi/IntrinsicFeature> ;
                                        rdfs:comment "The rhythmic structure and stylistic elements of a document's text" ;
                                        rdfs:label "metre and style" .


###  https://w3id.org/sebi/mock
<https://w3id.org/sebi/mock> rdf:type owl:NamedIndividual ,
                                      <https://w3id.org/sebi/Intention> ;
                             rdfs:comment "To imitate or mimic something in a way that is often intended to ridicule or criticize, commonly used as a form of satire or parody." ;
                             rdfs:label "mock" .


###  https://w3id.org/sebi/nationalism_patriotism
<https://w3id.org/sebi/nationalism_patriotism> rdf:type owl:NamedIndividual ,
                                                        <https://w3id.org/sebi/Intention> ;
                                               rdfs:comment "The production of documents that promote national pride or loyalty, sometimes through the embellishment or fabrication of facts, to support patriotic narratives." ;
                                               rdfs:label "nationalism / patriotism" .


###  https://w3id.org/sebi/original_document
<https://w3id.org/sebi/original_document> rdf:type owl:NamedIndividual ,
                                                   <https://w3id.org/sebi/Provenance> ;
                                          rdfs:comment "The initial version of a document" ;
                                          rdfs:label "original document" .


###  https://w3id.org/sebi/orthography
<https://w3id.org/sebi/orthography> rdf:type owl:NamedIndividual ,
                                             <https://w3id.org/sebi/IntrinsicFeature> ;
                                    rdfs:comment "The conventional spelling system of a document's language" ;
                                    rdfs:label "orthography" .


###  https://w3id.org/sebi/presence
<https://w3id.org/sebi/presence> rdf:type owl:NamedIndividual ,
                                          <https://w3id.org/sebi/Evaluation> ;
                                 rdfs:comment "The existence of specific a feature in a document" ;
                                 rdfs:label "presence" .


###  https://w3id.org/sebi/profit
<https://w3id.org/sebi/profit> rdf:type owl:NamedIndividual ,
                                        <https://w3id.org/sebi/Intention> ;
                               rdfs:comment "The creation or manipulation of documents to falsely represent financial gain, typically to deceive stakeholders or inflate the perceived success of an entity." ;
                               rdfs:label "profit" .


###  https://w3id.org/sebi/reliability
<https://w3id.org/sebi/reliability> rdf:type owl:NamedIndividual ,
                                             <https://w3id.org/sebi/Evaluation> ;
                                    rdfs:comment "The dependability of a document based on its features and Evaluations." ;
                                    rdfs:label "reliability" .


###  https://w3id.org/sebi/sigillum_or_seal
<https://w3id.org/sebi/sigillum_or_seal> rdf:type owl:NamedIndividual ,
                                                  <https://w3id.org/sebi/ExtrinsicFeature> ;
                                         rdfs:comment "An official mark or seal found on documents" ;
                                         rdfs:label "sigillum or seal" .


###  https://w3id.org/sebi/veridicality
<https://w3id.org/sebi/veridicality> rdf:type owl:NamedIndividual ,
                                              <https://w3id.org/sebi/Evaluation> ;
                                     rdfs:comment "The truthfulness and accuracy of a document's information." ;
                                     rdfs:label "veridicality" .


###  Generated by the OWL API (version 5.1.18) https://github.com/owlcs/owlapi/
